Weidenbach_Book/IsaSAT/IsaSAT_Inprocessing_LLVM.thy
@@ -7,9 +7,6 @@ theory IsaSAT_Inprocessing_LLVM
     IsaSAT_Simplify_Pure_Literals_LLVM
 begin
 
-no_notation WB_More_Refinement.fref (\<open>[_]\<^sub>f _ \<rightarrow> _\<close> [0,60,60] 60)
-no_notation WB_More_Refinement.freft (\<open>_ \<rightarrow>\<^sub>f _\<close> [60,60] 60)
-
 sepref_register 0 1
 
 sepref_register mop_arena_update_lit isa_pure_literal_count_occs_wl
