Weidenbach_Book/IsaSAT/IsaSAT_Simplify_Forward_Subsumption_LLVM.thy
@@ -9,9 +9,6 @@ theory IsaSAT_Simplify_Forward_Subsumption_LLVM
     IsaSAT_LBD_LLVM
 begin
 
-no_notation WB_More_Refinement.fref (\<open>[_]\<^sub>f _ \<rightarrow> _\<close> [0,60,60] 60)
-no_notation WB_More_Refinement.freft (\<open>_ \<rightarrow>\<^sub>f _\<close> [60,60] 60)
-
 lemma incr_forward_subsumed_st_alt_def: \<open>incr_forward_subsumed_st S = (
   let (stats, S) = extract_stats_wl_heur S; stats = incr_forward_subsumed stats in
     update_stats_wl_heur stats S
